theories/reactive/utp_rea_prog.thy
@@ -588,7 +588,7 @@ subsection \<open> Stateful Reactive specifications \<close>
 definition rea_st_rel :: "'s hrel \<Rightarrow> ('s, 't::trace, '\<alpha>, '\<beta>) rel_rsp" ("[_]\<^sub>S") where
 [upred_defs]: "rea_st_rel b = (\<lceil>b\<rceil>\<^sub>S \<and> $tr\<acute> =\<^sub>u $tr)"
 
-definition rea_st_rel' :: "'s hrel \<Rightarrow> ('s, 't::trace, '\<alpha>, '\<beta>) rel_rsp" ("[_]\<^sub>S'") where
+definition rea_st_rel' :: "'s hrel \<Rightarrow> ('s, 't::trace, '\<alpha>, '\<beta>) rel_rsp" ("[_]\<^sub>S''") where
 [upred_defs]: "rea_st_rel' b = R1(\<lceil>b\<rceil>\<^sub>S)"
 
 definition rea_st_cond :: "'s upred \<Rightarrow> ('s, 't::trace, '\<alpha>, '\<beta>) rel_rsp" ("[_]\<^sub>S\<^sub><") where
