utp/utp_rel_laws.thy
@@ -747,9 +747,9 @@ proof -
     by auto
   moreover have "(\<Sqinter>i. P(i)) = \<Sqinter> (P ` UNIV)"
     by (blast)
-  moreover have "\<Sqinter> (P ` insert 0 {1..}) = P(0) \<sqinter> SUPREMUM {1..} P"
+  moreover have "\<Sqinter> (P ` insert 0 {1..}) = P(0) \<sqinter> \<Sqinter> (P ` {1..})"
     by (simp)
-  moreover have "SUPREMUM {1..} P = (\<Sqinter>i. P(i+1))"
+  moreover have "\<Sqinter> (P ` {1..}) = (\<Sqinter>i. P(i+1))"
     by (simp add: atLeast_Suc_greaterThan greaterThan_0)
   ultimately show ?thesis
     by (simp only:)
